Simple prefilter optimization (#112)
* Extract the first character from an expr

* Add OptimizationInfo

* Use optimization info in search

* Prove the soundness and completeness of Iterator.find

* Prove that findStart preserves completeness

correctness/RegexCorrectness/Regex/Basic.lean
@@ -4,6 +4,7 @@ import RegexCorrectness.NFA.Compile
 import RegexCorrectness.Syntax.Ast
 import RegexCorrectness.Backtracker
 import RegexCorrectness.VM
+import RegexCorrectness.Regex.OptimizationInfo
 
 set_option autoImplicit false
 
@@ -17,9 +18,14 @@ def IsSearchRegex (re : Regex) : Prop :=
   ∃ e : Expr,
     re.nfa = NFA.compile (.group 0 e) ∧
     Expr.Disjoint (.group 0 e) ∧
-    re.maxTag = re.nfa.maxTag
+    re.maxTag = re.nfa.maxTag ∧
+    re.optimizationInfo = .fromExpr (.group 0 e)
 
 namespace IsSearchRegex
+
+theorem of_fromExpr {e : Expr} (h : Expr.Disjoint (.group 0 e)) : IsSearchRegex (.fromExpr (.group 0 e)) := by
+  simp [fromExpr]
+  exact ⟨e, rfl, h, rfl, rfl⟩
 
 theorem of_parse {s : String} {re : Regex} (h : Regex.parse s = .ok re) :
   IsSearchRegex re := by
@@ -31,7 +37,8 @@ theorem of_parse {s : String} {re : Regex} (h : Regex.parse s = .ok re) :
     have ⟨e, eq⟩ := Regex.Syntax.Parser.Ast.toRegex_group_of_group ast
     have disj : Expr.Disjoint (.group 0 e) :=
       eq ▸ Regex.Syntax.Parser.Ast.toRegex_disjoint (.group ast)
-    exact ⟨e, by simp [←h, eq], disj, by simp [←h]⟩
+    rw [←h, eq]
+    exact of_fromExpr disj
   | .error e => simp [Except.map] at h
 
 noncomputable def inner {re : Regex} (s : IsSearchRegex re) : Expr :=
@@ -47,7 +54,10 @@ theorem disj {re : Regex} (s : IsSearchRegex re) : Expr.Disjoint s.expr :=
   s.choose_spec.2.1
 
 theorem maxTag_eq {re : Regex} (s : IsSearchRegex re) : re.maxTag = re.nfa.maxTag :=
-  s.choose_spec.2.2
+  s.choose_spec.2.2.1
+
+theorem optimizationInfo_eq {re : Regex} (s : IsSearchRegex re) : re.optimizationInfo = .fromExpr s.expr :=
+  s.choose_spec.2.2.2
 
 theorem le_maxTag {re : Regex} (s : IsSearchRegex re) : 1 ≤ re.maxTag := by
   simp [s.maxTag_eq]
@@ -64,10 +74,12 @@ theorem captureNextBuf_soundness' {re bufferSize it matched} (h : re.captureNext
     EquivMaterializedUpdate (materializeRegexGroups groups) matched := by
   if bt : re.useBacktracker then
     simp [Regex.captureNextBuf, bt, s.nfa_eq] at h
-    exact Backtracker.captureNext_soundness s.disj h v
+    have ⟨it', it'', groups, eqs, le, c, eqv⟩ := Backtracker.captureNext_soundness s.disj h (OptimizationInfo.valid_findStart_of_valid v)
+    exact ⟨it', it'', groups, by grind, Nat.le_trans OptimizationInfo.findStart_le_pos le, c, eqv⟩
   else
     simp [Regex.captureNextBuf, bt, s.nfa_eq] at h
-    exact VM.captureNext_soundness s.disj h v
+    have ⟨it', it'', groups, eqs, le, c, eqv⟩ := VM.captureNext_soundness s.disj h (OptimizationInfo.valid_findStart_of_valid v)
+    exact ⟨it', it'', groups, by grind, Nat.le_trans OptimizationInfo.findStart_le_pos le, c, eqv⟩
 
 theorem captureNextBuf_soundness {re bufferSize it matched} (h : re.captureNextBuf bufferSize it = .some matched)
   (s : IsSearchRegex re) (v : it.Valid) (le : 2 ≤ bufferSize) :
@@ -90,18 +102,29 @@ theorem captureNextBuf_soundness {re bufferSize it matched} (h : re.captureNextB
     simp [h₁, h₂] at eqv
     exact ⟨eqv.1.symm, eqv.2.symm⟩
 
+theorem captureNextBuf_completeness' {re bufferSize it} (h : re.captureNextBuf bufferSize it = .none)
+  (s : IsSearchRegex re) (v : it.Valid) (it' it'' : Iterator) (groups : Data.CaptureGroups)
+  (eqs : it'.toString = it.toString) (le : it.pos ≤ it'.pos) (c : s.expr.Captures it' it'' groups) :
+  False := by
+  have : it'.pos < (re.optimizationInfo.findStart it).pos ∨ (re.optimizationInfo.findStart it).pos ≤ it'.pos :=
+    Nat.lt_or_ge _ _
+  cases this with
+  | inl lt => exact OptimizationInfo.findStart_completeness s.optimizationInfo_eq v eqs le lt c
+  | inr ge =>
+    if bt : re.useBacktracker then
+      simp [Regex.captureNextBuf, bt, s.nfa_eq] at h
+      exact Backtracker.captureNext_completeness' h (OptimizationInfo.valid_findStart_of_valid v) it' it'' groups (by grind) ge c
+    else
+      simp [Regex.captureNextBuf, bt, s.nfa_eq] at h
+      exact VM.captureNext_completeness' h (OptimizationInfo.valid_findStart_of_valid v) it' it'' groups (by grind) ge c
+
 theorem captureNextBuf_completeness {re bufferSize it} (h : re.captureNextBuf bufferSize it = .none)
   (s : IsSearchRegex re) (v : it.Valid) :
   ¬∃ it' it'' groups,
     it'.toString = it.toString ∧
     it.pos ≤ it'.pos ∧
     s.expr.Captures it' it'' groups := by
-  if bt : re.useBacktracker then
-    simp [Regex.captureNextBuf, bt, s.nfa_eq] at h
-    exact Backtracker.captureNext_completeness h v
-  else
-    simp [Regex.captureNextBuf, bt, s.nfa_eq] at h
-    exact VM.captureNext_completeness h v
+  grind [captureNextBuf_completeness']
 
 theorem searchNext_some {re it str} (h : re.searchNext it = .some str)
   (s : IsSearchRegex re) (v : it.Valid) :
