regex/Regex/Data/Expr/Basic.lean
@@ -1,0 +1,21 @@
+import Regex.Data.Anchor
+import Regex.Data.Classes
+
+namespace Regex.Data
+
+/--
+An inductive type that represents a regular expression.
+-/
+inductive Expr : Type where
+  | empty : Expr
+  | epsilon : Expr
+  | anchor : Anchor → Expr
+  | char : Char → Expr
+  | group : Nat → Expr → Expr
+  | alternate : Expr → Expr → Expr
+  | concat : Expr → Expr → Expr
+  | star : Expr → Expr
+  | classes : Classes → Expr
+deriving Repr, Inhabited
+
+end Regex.Data
