regex/Regex/Data/Expr/Optimization.lean
@@ -1,0 +1,27 @@
+import Regex.Data.Expr.Basic
+
+namespace Regex.Data.Expr
+
+def nullOnly (expr : Expr) : Bool :=
+  match expr with
+  | .empty | .epsilon | .anchor _ => true
+  | .char _ | .classes _ => false
+  | .group _ e => e.nullOnly
+  | .concat e₁ e₂ => e₁.nullOnly && e₂.nullOnly
+  | .alternate e₁ e₂ => e₁.nullOnly && e₂.nullOnly
+  | .star e => e.nullOnly
+
+def firstChar (expr : Expr) : Option Char :=
+  match expr with
+  | .empty | .epsilon | .anchor _ => .none
+  | .char c => .some c
+  | .classes _ => .none
+  | .group _ e => e.firstChar
+  | .concat e₁ e₂ => if e₁.nullOnly then e₂.firstChar else e₁.firstChar
+  | .alternate e₁ e₂ => do
+    let c₁ ← e₁.firstChar
+    let c₂ ← e₂.firstChar
+    if c₁ = c₂ then .some c₁ else .none
+  | .star _ => .none
+
+end Regex.Data.Expr
